\textbf{\# For the prediction:} \label{appendix.sec.bootstrap-prediction}
%
\begin{equation*}
    \mathbb{P}_{t} \paren*{ X_{t+1} \in dx_{t+1} \vert Y_{0:t} = y_{0:t} }
\end{equation*}
%
According to Eq. \eqref{eq.forward-recursion.extension} of extension:
%
\begin{equation*}
    \mathbb{Q}_{t-1} \paren*{dx_{t-1:t}} =
        \mathbb{Q}_{t-1} \paren*{dx_{t-1}}
        \cdot M_{t} \paren*{x_{t-1}, dx_{t}}
\end{equation*}
%
, which leads to
%
\begin{align*}
    \int_{x_{t-1} \in \mathcal{X}} \mathbb{P}_{t-1}
        \paren*{ X_{t-1:t} \in dx_{t-1:t} \vert Y_{0:t-1} = y_{0:t-1}}
    &=
        \int_{x_{t-1} \in \mathcal{X}} \mathbb{P}_{t-1}
        \paren*{ X_{t-1} \in dx_{t-1} \vert Y_{0:t-1} = y_{0:t-1}}
        \cdot P_{t} \paren*{x_{t-1}, dx_{t}}
    \\[1.5ex]
    \mathbb{P}_{t-1}
        \paren*{ X_{t} \in dx_{t} \vert Y_{0:t-1} = y_{0:t-1}}
    &=
        \int_{x_{t-1} \in \mathcal{X}} \mathbb{P}_{t-1}
        \paren*{ X_{t-1} \in dx_{t-1} \vert Y_{0:t-1} = y_{0:t-1}}
        \cdot P_{t} \paren*{x_{t-1}, dx_{t}}
\end{align*}
