\textbf{\# Extension}

According to Eq. \eqref{eq.FK.02}:
%
\begin{equation*}
    \mathbb{Q}_{t-1} \paren*{dx_{0:t}} =
        \dfrac{1}{L_{t-1}} \,
        G_{0} \paren*{x_{0}} \cdot \bracket*{
            \prod_{s = 1}^{{t-1}} G_{s} \paren*{x_{s - 1}, x_{s}}
        }
        \cdot \mathbb{M}_{t} \paren*{dx_{0:t}}
\end{equation*}
%
, with
%
\begin{equation*}
    \mathbb{Q}_{t-1} \paren*{dx_{0:t-1}} =
        \dfrac{1}{L_{t-1}} \,
        G_{0} \paren*{x_{0}} \cdot \bracket*{
            \prod_{s = 1}^{{t-1}} G_{s} \paren*{x_{s - 1}, x_{s}}
        }
        \cdot \mathbb{M}_{t-1} \paren*{dx_{0:t-1}}
\end{equation*}
%
, we have
%
\begin{alignat}{3}
    & \Rightarrow &
    \mathbb{Q}_{t-1} \paren*{dx_{0:t}} &=
        \mathbb{Q}_{t-1} \paren*{dx_{0:t-1}}
        \cdot M_{t} \paren*{x_{t-1}, dx_{t}}
    \nonumber \\[1.5ex] & \Rightarrow
    \int_{x_{0:t-2} \in \mathcal{X}^{t-1}} &
        \mathbb{Q}_{t-1} \paren*{dx_{0:t}} &=
        \int _{x_{0:t-2} \in \mathcal{X}^{t-1}}
        \mathbb{Q}_{t-1} \paren*{dx_{0:t-1}}
        \cdot M_{t} \paren*{x_{t-1}, dx_{t}}
    \nonumber \\[1.5ex] & \Rightarrow &
        \mathbb{Q}_{t-1} \paren*{dx_{t-1:t}} &=
            \mathbb{Q}_{t-1} \paren*{dx_{t-1}}
            \cdot M_{t} \paren*{x_{t-1}, dx_{t}}
    \label{appendix.eq.forward-recursion.extension}
\end{alignat}